# 3021

## Question

(Omitted)

## Solution 

The description is long but it comes down to counting tuples `(a, b)` with `1 <= a <= n` and `1 <= b <= m` such that `a + b` is odd.

Since of the sum of two integers is odd if and only if one is odd and the other is even, so we just need to
* count the tuple where `a` is even and `b` is odd
* count the tuple where `a` is odd and `b` is even

Naively, this would yield `a * (b - b // 2) + (a - a // 2) * b`. However, we can further simplify this: if `a = 2 x + c` and `b = 2 y + d` with `c, d in (0, 1)`, substituting in the expression, the result is `2 x y + x d + y c`. At the same time, a bit computation implies `a * b = 4 x y + 2 x d + 2 y c + c d`. By assumption `c d <= 1`, so `(a * b) // 2` yields exactly the same expression.

While this does yield shorter asm code, the actual performance gain seems minimal, as the original code is already quite fast.

